library/init/meta/tactic.lean
@@ -733,11 +733,15 @@ do gs ← get_goals, focus_aux ts gs []
 
 meta def focus1 {α} (tac : tactic α) : tactic α :=
 do g::gs ← get_goals,
-   set_goals [g],
-   a ← tac,
-   gs' ← get_goals,
-   set_goals (gs' ++ gs),
-   return a
+   match gs with
+   | [] := tac
+   | _  := do
+      set_goals [g],
+      a ← tac,
+      gs' ← get_goals,
+      set_goals (gs' ++ gs),
+      return a
+   end
 
 private meta def all_goals_core (tac : tactic unit) : list expr → list expr → tactic unit
 | []        ac := set_goals ac
